add Parse tree version of lemma

Roos/chomsky_schuetzenberger.thy
@@ -1,5 +1,5 @@
 theory chomsky_schuetzenberger
-  imports  "../CFG" "../CFL" Chain "$AFP/Regular-Sets/Regexp_Constructions" "$AFP/Regular-Sets/Regular_Set"
+  imports  "../CFG" "../CFL" "../Parse_Tree" Chain "$AFP/Regular-Sets/Regexp_Constructions" "$AFP/Regular-Sets/Regular_Set"
 begin
 
 text \<open>This file contains all the constructions needed for the chomsky-schuetzenberger theorem.
@@ -899,10 +899,11 @@ text\<open>The transformation of old productions to new productions used in the 
 fun transform_production :: "('n, 't) prod \<Rightarrow> 
 ('n, bracket \<times> ('n,'t) prod \<times> version) prod" where
   \<open>  transform_production (A, [Nt B, Nt C]) =    
-        (A, [ Tm (Op, ((A, [Nt B, Nt C]), One)), Nt B, Tm (Cl, ((A, [Nt B, Nt C]), One)), Tm (Op, ((A, [Nt B, Nt C]), Two)), Nt C, Tm (Cl, ((A, [Nt B, Nt C]), Two))  ])\<close> | 
+        (A, [ Tm (Op, (A, [Nt B, Nt C]), One), Nt B, Tm (Cl, (A, [Nt B, Nt C]), One), Tm (Op, (A, [Nt B, Nt C]), Two), Nt C, Tm (Cl, (A, [Nt B, Nt C]), Two)  ])  \<close> | 
 
 \<open> transform_production (A, [Tm a])  = 
- (A, [ Tm (Op, ((A, [Tm a]),One)),       Tm (Cl, ((A, [Tm a]), One)), Tm (Op, ((A, [Tm a]), Two)),       Tm (Cl, ((A, [Tm a]), Two))  ]) \<close> | 
+        (A, [ Tm (Op, (A, [Tm a]),One),       Tm (Cl, (A, [Tm a]), One), Tm (Op, ((A, [Tm a]), Two)),       Tm (Cl, (A, [Tm a]), Two)  ]) \<close> | 
+
 \<open>transform_production (A, _) = (A, [])\<close>
 
 
@@ -943,8 +944,24 @@ definition CNF_rule :: "('n,'t) prod \<Rightarrow> bool" where
 lemma transform_production_CNF: \<open>CNF_rule p \<Longrightarrow> (\<exists>A B C. transform_production p = (A, [ Tm [\<^sub>p\<^sup>1 , Nt B, Tm ]\<^sub>p\<^sup>1 , Tm [\<^sub>p\<^sup>2 , Nt C, Tm ]\<^sub>p\<^sup>2   ]) \<and> p = (A, [Nt B, Nt C])) \<or> (\<exists>A a. transform_production p = (A, [ Tm [\<^sub>p\<^sup>1,       Tm ]\<^sub>p\<^sup>1 , Tm [\<^sub>p\<^sup>2 ,       Tm ]\<^sub>p\<^sup>2   ]) \<and> p = (A, [Tm a]) )\<close>
   unfolding CNF_rule_def by auto
 
+lemma transform_production_when_CNF: 
+assumes \<open>CNF_rule p\<close>
+shows \<open>\<exists>A B C a.    
+ p = (A, [Nt B, Nt C]) \<and> transform_production p = (A, [ Tm (Op, (A, [Nt B, Nt C]), One), Nt B, Tm (Cl, ((A, [Nt B, Nt C]), One)), Tm (Op, (A, [Nt B, Nt C]), Two), Nt C, Tm (Cl, (A, [Nt B, Nt C]), Two)  ])  
+\<or>
+ p = (A, [Tm a])       \<and> transform_production p =   (A, [ Tm (Op, (A, [Tm a]),One),       Tm (Cl, (A, [Tm a]), One), Tm (Op, (A, [Tm a]), Two),       Tm (Cl, (A, [Tm a]), Two)  ])  
+\<close>
+using assms unfolding CNF_rule_def by auto
 
 
+lemma transform_production_when_CNF':
+assumes \<open>CNF_rule (A,r)\<close>
+shows \<open>\<exists>B C a.    
+ (A,r) = (A, [Nt B, Nt C]) \<and> transform_production (A,r) = (A, [ Tm (Op, (A, [Nt B, Nt C]), One), Nt B, Tm (Cl, ((A, [Nt B, Nt C]), One)), Tm (Op, (A, [Nt B, Nt C]), Two), Nt C, Tm (Cl, (A, [Nt B, Nt C]), Two)  ])  
+\<or>
+ (A,r) = (A, [Tm a])       \<and> transform_production (A,r) =   (A, [ Tm (Op, (A, [Tm a]),One),       Tm (Cl, (A, [Tm a]), One), Tm (Op, (A, [Tm a]), Two),       Tm (Cl, (A, [Tm a]), Two)  ])  
+\<close>
+using transform_production_when_CNF fst_transform_production using assms by blast
 
 
 
@@ -964,6 +981,75 @@ lemma CNF_existence :
   assumes \<open>CFL.cfl TYPE('a) L\<close>
   shows \<open>\<exists>P S::'a. L = Lang P S \<and> (\<forall>p \<in> P. CNF_rule p)\<close> (* TODO start symbol not on the right side*)
   sorry
+
+
+
+
+
+
+
+
+
+
+
+
+
+
+
+
+
+
+
+
+
+
+
+
+
+
+
+
+
+
+
+
+
+
+
+
+
+
+
+
+
+
+
+
+
+
+
+
+
+
+
+
+
+
+
+
+
+
+
+
+
+
+
+
+
+
+
+
+
 
 
 
@@ -1979,6 +2065,295 @@ qed
 
 
   
+
+
+
+
+
+
+
+
+
+
+
+
+
+
+
+
+
+
+
+
+
+
+
+
+
+
+
+
+
+
+
+
+
+
+
+
+
+
+
+
+
+
+
+
+
+
+
+
+
+section\<open>Transformation of a parse tree\<close>
+
+
+abbreviation \<open>prod_rhs ts \<equiv> map root ts\<close>
+
+fun transform_tree :: \<open>('n,'t) tree \<Rightarrow> ('n, bracket \<times> ('n \<times> ('n, 't) sym list) \<times> version) tree\<close> where
+\<open>transform_tree (Sym (Nt A)) = (Sym (Nt A))\<close> | 
+\<open>transform_tree (Sym (Tm a)) = (Sym (Tm (Op, ((SOME A. True, [Tm a]), One))))\<close> | 
+\<open>transform_tree (Prod A [Sym (Tm a)]) =             (Prod A [ Sym (Tm (Op, (A, [Tm a]),One)),       Sym(Tm (Cl, (A, [Tm a]), One)), Sym (Tm (Op, (A, [Tm a]), Two)),       Sym(Tm (Cl, (A, [Tm a]), Two))  ])\<close> | 
+\<open>transform_tree (Prod A [Sym (Nt B), Sym (Nt C)]) =  (Prod A [Sym (Tm (Op, (A, [Nt B, Nt C]), One)), Sym (Nt B), Sym (Tm (Cl, ((A, [Nt B, Nt C]), One))), Sym (Tm (Op, (A, [Nt B, Nt C]), Two)), Sym (Nt C), Sym (Tm (Cl, (A, [Nt B, Nt C]), Two))  ])\<close> | 
+\<open>transform_tree (Prod A [Prod B tB, Sym (Nt C)]) =   (Prod A [Sym (Tm (Op, (A, [Nt B, Nt C]), One)), transform_tree (Prod B tB), Sym (Tm (Cl, ((A, [Nt B, Nt C]), One))), Sym (Tm (Op, (A, [Nt B, Nt C]), Two)), Sym (Nt C), Sym (Tm (Cl, (A, [Nt B, Nt C]), Two))  ])  \<close> | 
+\<open>transform_tree (Prod A [Sym (Nt B), Prod C tC]) =   (Prod A [Sym (Tm (Op, (A, [Nt B, Nt C]), One)), Sym (Nt B), Sym (Tm (Cl, ((A, [Nt B, Nt C]), One))), Sym (Tm (Op, (A, [Nt B, Nt C]), Two)), transform_tree (Prod C tC), Sym (Tm (Cl, (A, [Nt B, Nt C]), Two))  ])\<close> | 
+\<open>transform_tree (Prod A [Prod B tB, Prod C tC]) =   (Prod A [Sym (Tm (Op, (A, [Nt B, Nt C]), One)), transform_tree (Prod B tB), Sym (Tm (Cl, ((A, [Nt B, Nt C]), One))), Sym (Tm (Op, (A, [Nt B, Nt C]), Two)), transform_tree (Prod C tC), Sym (Tm (Cl, (A, [Nt B, Nt C]), Two))  ])\<close> | 
+\<open>transform_tree (Prod A y) = (Prod A [])\<close>
+
+lemma root_of_transform_tree[intro]: \<open>root t = Nt X \<Longrightarrow> root (transform_tree t) = Nt X\<close>
+apply(induction t rule: transform_tree.induct) by auto 
+
+
+lemma transform_tree_correct:
+fixes P
+defines \<open>P' == transform_production ` P\<close>
+assumes \<open>parse_tree P t \<and> fringe t = w\<close>
+and \<open>\<And>p. p \<in> P \<Longrightarrow> CNF_rule p\<close>
+shows \<open>parse_tree P' (transform_tree t)  \<and>  the_hom_ext (fringe (transform_tree t)) = w\<close>
+using assms proof(induction t arbitrary: w)
+  case (Sym x)
+  from Sym have pt: \<open>parse_tree P (Sym x)\<close> and \<open>fringe (Sym x) = w\<close> by blast+
+  from Sym have CNF: \<open>\<And>p. p \<in> P \<Longrightarrow> CNF_rule p\<close> by blast
+  then show ?case 
+  proof(cases x)
+    case (Nt x1)
+    then have \<open>transform_tree (Sym x) = (Sym (Nt x1))\<close> by simp 
+    then show ?thesis using Sym by (metis Nt Parse_Tree.fringe.simps(1) Parse_Tree.parse_tree.simps(1) the_hom_ext_keep_var)
+  next
+    case (Tm x2)
+    then obtain a where \<open>transform_tree (Sym x) = (Sym (Tm (Op, ((SOME A. True, [Tm a]), One))))\<close> by simp
+    then have \<open>fringe ... = [(Tm (Op, ((SOME A. True, [Tm a]), One)))]\<close> by simp
+    then have \<open>the_hom_ext ... = [Tm a]\<close> by simp
+    then have \<open>... = w\<close> using Sym using Tm \<open>transform_tree (Sym x) = Sym (Tm [\<^bsub>(SOME A. True, [Tm a])\<^esub>\<^sup>1 )\<close> by force
+    then show ?thesis  using Sym by (metis Parse_Tree.parse_tree.simps(1) \<open>fringe (Sym (Tm [\<^bsub>(SOME A. True, [Tm a])\<^esub>\<^sup>1 )) = [Tm [\<^bsub>(SOME A. True, [Tm a])\<^esub>\<^sup>1 ]\<close> \<open>the_hom_ext [Tm [\<^bsub>(SOME A. True, [Tm a])\<^esub>\<^sup>1 ] = [Tm a]\<close> \<open>transform_tree (Sym x) = Sym (Tm [\<^bsub>(SOME A. True, [Tm a])\<^esub>\<^sup>1 )\<close>)
+  qed
+next
+  case (Prod A ts)
+  from Prod have pt: \<open>parse_tree P (Prod A ts)\<close> and fr: \<open>fringe (Prod A ts) = w\<close> by blast+
+  from Prod have IH: \<open>\<And>x2a w'. \<lbrakk>x2a \<in> set ts; parse_tree P x2a \<and> fringe x2a = w'\<rbrakk> \<Longrightarrow> parse_tree P' (transform_tree x2a) \<and> the_hom_ext (fringe (transform_tree x2a)) = w'\<close> using P'_def by blast
+  
+  from pt have \<open>(A, map root ts) \<in> P\<close> by simp
+  then have \<open>CNF_rule (A, map root ts)\<close> using Prod.prems(2) by blast
+
+  then obtain B C a where 
+      def: \<open>(A, prod_rhs ts) = (A, [Nt B, Nt C]) \<and> transform_production (A, prod_rhs ts) = (A, [Tm [\<^bsub>(A, [Nt B, Nt C])\<^esub>\<^sup>1 , Nt B, Tm ]\<^bsub>(A, [Nt B, Nt C])\<^esub>\<^sup>1, Tm [\<^bsub>(A, [Nt B, Nt C])\<^esub>\<^sup>2, Nt C, Tm ]\<^bsub>(A, [Nt B, Nt C])\<^esub>\<^sup>2 ]) 
+\<or>
+       (A, prod_rhs ts) = (A, [Tm a]) \<and> transform_production (A, prod_rhs ts) = (A, [Tm [\<^bsub>(A, [Tm a])\<^esub>\<^sup>1 , Tm ]\<^bsub>(A, [Tm a])\<^esub>\<^sup>1, Tm [\<^bsub>(A, [Tm a])\<^esub>\<^sup>2, Tm ]\<^bsub>(A, [Tm a])\<^esub>\<^sup>2 ])\<close> using transform_production_when_CNF' assms(3) by meson
+  then obtain e1 e2 e3 where ei_def: \<open>ts = [e1] \<or> ts = [e2, e3]\<close> by blast  
+  obtain tB tC where 
+\<open>(ts = [Sym (Tm a)] \<and> prod_rhs ts = [Tm a]) 
+\<or> 
+prod_rhs ts = [Nt B, Nt C]  \<and>  (ts = [Sym (Nt B), Sym (Nt C)] \<or> ts = [Prod B tB, Sym (Nt C)] \<or> ts = [Sym (Nt B), Prod C tC] \<or> ts = [Prod B tB, Prod C tC])\<close>
+          apply(rule disjE[OF def]) 
+          using root.elims root.simps \<open>CNF_rule (A, prod_rhs ts)\<close> apply (smt (verit, ccfv_threshold) CFG.sym.inject(1) Cons_eq_map_D Product_Type.prod.inject map_is_Nil_conv)
+          using root.elims root.simps \<open>CNF_rule (A, prod_rhs ts)\<close> 
+          proof -
+            assume a1: "(A, prod_rhs ts) = (A, [Tm a]) \<and> transform_production (A, prod_rhs ts) = (A, [Tm [\<^bsub>(A, [Tm a])\<^esub>\<^sup>1 , Tm ]\<^bsub>(A, [Tm a])\<^esub>\<^sup>1, Tm [\<^bsub>(A, [Tm a])\<^esub>\<^sup>2, Tm ]\<^bsub>(A, [Tm a])\<^esub>\<^sup>2 ])"
+            assume a2: "\<And>tB tC. ts = [Sym (Tm a)] \<and> prod_rhs ts = [Tm a] \<or> prod_rhs ts = [Nt B, Nt C] \<and> (ts = [Sym (Nt B), Sym (Nt C)] \<or> ts = [Prod B tB, Sym (Nt C)] \<or> ts = [Sym (Nt B), Prod C tC] \<or> ts = [Prod B tB, Prod C tC]) \<Longrightarrow> thesis"
+            have f3: "prod_rhs [] = []"
+              by force
+            have "[] \<noteq> ts"
+              using a1 by force
+            then show ?thesis
+              using f3 a2 a1 by (metis (no_types) CFG.sym.simps(4) List.last.simps List.list.simps(9) Parse_Tree.root.elims Product_Type.prod.inject ei_def not_Cons_self2)
+          qed
+
+  
+  then consider (Tm) \<open>ts = [Sym (Tm a)] \<and> prod_rhs ts = [Tm a]\<close> | (Nt_Nt) \<open>prod_rhs ts = [Nt B, Nt C] \<and> ts = [Sym (Nt B), Sym (Nt C)]\<close> | (Prod_Nt) \<open>prod_rhs ts = [Nt B, Nt C] \<and> ts = [Prod B tB, Sym (Nt C)]\<close> | (Nt_Prod) \<open>prod_rhs ts = [Nt B, Nt C] \<and> ts = [Sym (Nt B), Prod C tC]\<close> | (Prod_Prod) \<open>prod_rhs ts = [Nt B, Nt C] \<and> ts = [Prod B tB, Prod C tC]\<close> by argo
+  then show ?case
+  proof(cases)
+    case Tm
+    then have ts_eq: \<open>ts = [Sym (Tm a)]\<close> and prod_rhs: \<open>prod_rhs ts = [Tm a]\<close> by blast+
+    then have \<open>transform_tree (Prod A ts) = (Prod A [ Sym (Tm (Op, (A, [Tm a]),One)),       Sym(Tm (Cl, (A, [Tm a]), One)), Sym (Tm (Op, (A, [Tm a]), Two)),       Sym(Tm (Cl, (A, [Tm a]), Two))  ])\<close> by simp
+    then have \<open>the_hom_ext (fringe (transform_tree (Prod A ts))) = [Tm a]\<close> by simp
+    also have \<open>... = w\<close> using fr unfolding ts_eq by auto
+    finally have \<open>the_hom_ext (fringe (transform_tree (Prod A ts))) = w\<close> .
+
+    moreover have \<open>parse_tree (P') (transform_tree (Prod A [Sym (Tm a)]))\<close> using pt prod_rhs unfolding P'_def by force 
+    ultimately show ?thesis unfolding ts_eq P'_def by blast
+  next
+    case Nt_Nt
+    then have ts_eq: \<open>ts = [Sym (Nt B), Sym (Nt C)]\<close>  and prod_rhs: \<open>prod_rhs ts = [Nt B, Nt C]\<close> by blast+
+    then have \<open>transform_tree (Prod A ts) = (Prod A [Sym (Tm (Op, (A, [Nt B, Nt C]), One)), Sym (Nt B), Sym (Tm (Cl, ((A, [Nt B, Nt C]), One))), Sym (Tm (Op, (A, [Nt B, Nt C]), Two)), Sym (Nt C), Sym (Tm (Cl, (A, [Nt B, Nt C]), Two))  ])\<close> by simp
+    then have \<open>the_hom_ext (fringe (transform_tree (Prod A ts))) = [ Nt B, Nt C  ]\<close> by simp
+    also have \<open>... = w\<close> using fr unfolding ts_eq by auto
+    finally have \<open>the_hom_ext (fringe (transform_tree (Prod A ts))) = w\<close> .
+
+    moreover have \<open>parse_tree (P') (transform_tree (Prod A [Sym (Nt B), Sym (Nt C)]))\<close> using pt prod_rhs unfolding P'_def by force
+    ultimately show ?thesis unfolding ts_eq by blast
+  next
+    case Prod_Nt
+    then have ts_eq: \<open>ts = [Prod B tB, Sym (Nt C)]\<close>  and prod_rhs: \<open>prod_rhs ts = [Nt B, Nt C]\<close> by blast+
+    then have transf_ts: \<open>transform_tree (Prod A ts) = (Prod A   [  Sym (Tm (Op, (A, [Nt B, Nt C]), One)),  transform_tree (Prod B tB),  Sym (Tm (Cl, ((A, [Nt B, Nt C]), One))),  Sym (Tm (Op, (A, [Nt B, Nt C]), Two)),   Sym (Nt C),   Sym (Tm (Cl, (A, [Nt B, Nt C]), Two))    ] )\<close> by simp
+    
+    then have frA: \<open>the_hom_ext (fringe (transform_tree (Prod A ts))) = the_hom_ext (fringe (transform_tree (Prod B tB))) @ [  Nt C  ]\<close> by simp
+
+    have ptB: \<open>parse_tree P (Prod B tB)\<close> using pt ts_eq by (meson List.list.set_intros(1) Parse_Tree.parse_tree.simps(2))
+    then have ptB: \<open>parse_tree (P') (transform_tree (Prod B tB))\<close> \<open>the_hom_ext (fringe (transform_tree (Prod B tB))) = fringe (Prod B tB)\<close>
+        using IH[of \<open>Prod B tB\<close> \<open>fringe (Prod B tB)\<close>] by (metis List.list.set_intros(1) assms(2) ts_eq)+
+
+    with frA have \<open>the_hom_ext (fringe (transform_tree (Prod A ts))) = fringe (Prod B tB) @ [Nt C]\<close> 
+        by presburger
+    also have \<open>... = fringe (Prod A [Prod B tB, Sym (Nt C)])\<close> 
+        using fringe.simps(2)[of A \<open>[Prod B tB, Sym (Nt C)]\<close>] 
+        by auto
+    also have \<open>... = fringe (Prod A ts)\<close> 
+        using ts_eq prod_rhs pt by blast
+    also have \<open>... = w\<close> 
+        using fr unfolding ts_eq by auto
+    finally have fin: \<open>the_hom_ext (fringe (transform_tree (Prod A ts))) = w\<close> .
+
+    have \<open>parse_tree (P') (transform_tree (Prod B tB)) \<and> (A, map root ts) \<in> P\<close> 
+        by (simp add: \<open>(A, prod_rhs ts) \<in> P\<close> ptB(1)) 
+    moreover have \<open>root (transform_tree (Prod B tB)) = Nt B\<close> 
+        apply(induction \<open>(Prod B tB)\<close> rule: transform_tree.induct) by auto
+    moreover have \<open>transform_production (A, prod_rhs ts) \<in> P'\<close> 
+        by (simp add: P'_def \<open>(A, prod_rhs ts) \<in> P\<close>)
+    ultimately have \<open>parse_tree (P') (transform_tree (Prod A ts))\<close> 
+        unfolding transf_ts ts_eq P'_def using ptB parse_tree.simps prod_rhs def by auto
+
+    then show ?thesis using fin by blast
+
+  next
+    case Nt_Prod
+    then have ts_eq: \<open>ts = [Sym (Nt B), Prod C tC]\<close>  and prod_rhs: \<open>prod_rhs ts = [Nt B, Nt C]\<close> by blast+
+    then have transf_ts: \<open>transform_tree (Prod A ts) = (Prod A   [  Sym (Tm (Op, (A, [Nt B, Nt C]), One)),  Sym (Nt B),  Sym (Tm (Cl, ((A, [Nt B, Nt C]), One))),  Sym (Tm (Op, (A, [Nt B, Nt C]), Two)),   transform_tree (Prod C tC),   Sym (Tm (Cl, (A, [Nt B, Nt C]), Two))    ] )\<close> by simp
+    
+    then have frA: \<open>the_hom_ext (fringe (transform_tree (Prod A ts))) = the_hom_ext ([  Nt B  ]@fringe (transform_tree (Prod C tC)))\<close> by simp
+
+    have ptC: \<open>parse_tree P (Prod C tC)\<close> using pt ts_eq by (meson List.list.set_intros(1,2) Parse_Tree.parse_tree.simps(2))
+
+    then have ptC: \<open>parse_tree (P') (transform_tree (Prod C tC))\<close> \<open>the_hom_ext (fringe (transform_tree (Prod C tC))) = fringe (Prod C tC)\<close>
+        using IH[of \<open>Prod C tC\<close> \<open>fringe (Prod C tC)\<close>] by (metis List.list.set_intros(1,2) ts_eq)+
+
+
+    with frA have \<open>the_hom_ext (fringe (transform_tree (Prod A ts))) = [Nt B] @ fringe (Prod C tC)\<close> by (metis the_hom_ext_hom the_hom_ext_keep_var)
+    also have \<open>... = fringe (Prod A [Sym (Nt B), Prod C tC])\<close> 
+        using fringe.simps(2)[of A \<open>[Sym (Nt B), Prod C tC]\<close>] 
+        by auto
+    also have \<open>... = fringe (Prod A ts)\<close> 
+        using ts_eq prod_rhs pt by blast
+    also have \<open>... = w\<close> 
+        using fr unfolding ts_eq by auto
+    finally have fin: \<open>the_hom_ext (fringe (transform_tree (Prod A ts))) = w\<close> .
+
+    have \<open>parse_tree (P') (transform_tree (Prod C tC)) \<and> (A, map root ts) \<in> P\<close> 
+        by (simp add: \<open>(A, prod_rhs ts) \<in> P\<close> ptC(1)) 
+    moreover have \<open>root (transform_tree (Prod C tC)) = Nt C\<close> 
+        apply(induction \<open>(Prod C tC)\<close> rule: transform_tree.induct) by auto
+    moreover have \<open>transform_production (A, prod_rhs ts) \<in> P'\<close> 
+        by (simp add: P'_def \<open>(A, prod_rhs ts) \<in> P\<close>)
+    ultimately have \<open>parse_tree (P') (transform_tree (Prod A ts))\<close> 
+        unfolding transf_ts ts_eq P'_def using ptC parse_tree.simps prod_rhs def by auto
+
+    then show ?thesis using fin by blast
+  next
+    case Prod_Prod
+    then have ts_eq: \<open>ts = [Prod B tB, Prod C tC]\<close>  and prod_rhs: \<open>prod_rhs ts = [Nt B, Nt C]\<close> by blast+
+    then have transf_ts: \<open>transform_tree (Prod A ts) = (Prod A   [  Sym (Tm (Op, (A, [Nt B, Nt C]), One)),  transform_tree (Prod B tB),  Sym (Tm (Cl, ((A, [Nt B, Nt C]), One))),  Sym (Tm (Op, (A, [Nt B, Nt C]), Two)),  transform_tree (Prod C tC),   Sym (Tm (Cl, (A, [Nt B, Nt C]), Two))    ] )\<close> by simp
+    
+    then have frA: \<open>the_hom_ext (fringe (transform_tree (Prod A ts))) = the_hom_ext (fringe (transform_tree (Prod B tB))) @ the_hom_ext (fringe (transform_tree (Prod C tC)))\<close> by simp
+
+    have ptB: \<open>parse_tree P (Prod B tB)\<close> using pt ts_eq by (meson List.list.set_intros(1) Parse_Tree.parse_tree.simps(2))
+    then have ptB: \<open>parse_tree (P') (transform_tree (Prod B tB))\<close> \<open>the_hom_ext (fringe (transform_tree (Prod B tB))) = fringe (Prod B tB)\<close>
+        using IH[of \<open>Prod B tB\<close> \<open>fringe (Prod B tB)\<close>] by (metis List.list.set_intros(1) assms(2) ts_eq)+
+
+    have ptC: \<open>parse_tree P (Prod C tC)\<close> using pt ts_eq by (meson List.list.set_intros(1,2) Parse_Tree.parse_tree.simps(2))
+    then have ptC: \<open>parse_tree (P') (transform_tree (Prod C tC))\<close> \<open>the_hom_ext (fringe (transform_tree (Prod C tC))) = fringe (Prod C tC)\<close>
+        using IH[of \<open>Prod C tC\<close> \<open>fringe (Prod C tC)\<close>] by (metis List.list.set_intros(1,2) ts_eq)+
+
+
+    from ptC ptB frA have \<open>the_hom_ext (fringe (transform_tree (Prod A ts))) = fringe (Prod B tB) @ fringe (Prod C tC)\<close> 
+        by presburger
+    also have \<open>... = fringe (Prod A [Prod B tB, Prod C tC])\<close> 
+        using fringe.simps(2)[of A \<open>[Prod B tB, Prod C tC]\<close>] 
+        by auto
+    also have \<open>... = fringe (Prod A ts)\<close> 
+        using ts_eq prod_rhs pt by blast
+    also have \<open>... = w\<close> 
+        using fr unfolding ts_eq by auto
+    finally have fin: \<open>the_hom_ext (fringe (transform_tree (Prod A ts))) = w\<close> .
+
+    have \<open>parse_tree (P') (transform_tree (Prod B tB)) \<and> (A, map root ts) \<in> P\<close> 
+        by (simp add: \<open>(A, prod_rhs ts) \<in> P\<close> ptB(1)) 
+    moreover have \<open>root (transform_tree (Prod B tB)) = Nt B\<close> 
+        apply(induction \<open>(Prod B tB)\<close> rule: transform_tree.induct) by auto
+    moreover have \<open>transform_production (A, prod_rhs ts) \<in> P'\<close> 
+        by (simp add: P'_def \<open>(A, prod_rhs ts) \<in> P\<close>)
+    moreover have \<open>parse_tree (P') (transform_tree (Prod C tC)) \<and> (A, map root ts) \<in> P\<close> 
+        by (simp add: \<open>(A, prod_rhs ts) \<in> P\<close> ptC(1)) 
+    moreover have \<open>root (transform_tree (Prod C tC)) = Nt C\<close> 
+        apply(induction \<open>(Prod C tC)\<close> rule: transform_tree.induct) by auto
+    moreover have \<open>transform_production (A, prod_rhs ts) \<in> P'\<close> 
+        by (simp add: P'_def \<open>(A, prod_rhs ts) \<in> P\<close>)
+    ultimately have \<open>parse_tree (P') (transform_tree (Prod A ts))\<close> 
+        unfolding transf_ts ts_eq P'_def using ptB parse_tree.simps prod_rhs def by auto
+
+    then show ?thesis using fin by blast
+  qed  
+qed
+
+
+
+lemma 
+assumes \<open>\<And>p. p \<in> P \<Longrightarrow> CNF_rule p\<close>
+and \<open>w \<in> Ders P S\<close>
+shows \<open>\<exists>w' \<in> Ders (transform_production ` P) S. w = the_hom_ext w'\<close>
+proof-
+
+from assms obtain t where t_def: \<open>parse_tree P t \<and> fringe t = w \<and> root t = Nt S\<close> using parse_tree_if_derives DersD sorry
+then have root_tr: \<open>root (transform_tree t) = Nt S\<close> by blast
+from t_def have \<open>parse_tree (transform_production ` P) (transform_tree t)  \<and>  the_hom_ext (fringe (transform_tree t)) = w\<close> using transform_tree_correct assms by blast
+with root_tr have \<open>fringe (transform_tree t) \<in> Ders (transform_production ` P) S \<and> w = the_hom_ext (fringe (transform_tree t))\<close> using fringe_steps_if_parse_tree by (metis DersI)
+then show ?thesis by blast
+qed
+
+
+
+
+
+
+
+
+
+
+
+
+
+
+
+
+
+
 
 
 
